qa/fv/Ragu/Circuits/Element/Square.lean
@@ -12,21 +12,20 @@ def Assumptions (_input : F p) := True
 def Spec (input : F p) (out : F p) :=
   out = input^2
 
-instance elaborated : ElaboratedCircuit (F p) field field where
-  main
+instance elaborated : ElaboratedCircuit (F p) field field main where
   output _ offset := varFromOffset field (offset + 2)
   localLength _ := 3
 
-theorem soundness : Soundness (F p) elaborated Assumptions Spec := by
+theorem soundness : Soundness (F p) (Input := field) (Output := field) main Assumptions Spec := by
   circuit_proof_start
   simp [circuit_norm, Mul.circuit, Mul.Assumptions, Mul.Spec] at h_holds ⊢
   rw [h_holds]
   ring
 
-theorem completeness : Completeness (F p) elaborated Assumptions := by
+theorem completeness : Completeness (F p) (Input := field) (Output := field) main Assumptions := by
   circuit_proof_start [Mul.circuit, Mul.Assumptions]
 
 def circuit : FormalCircuit (F p) field field :=
-  { elaborated with Assumptions, Spec, soundness, completeness }
+  { main := main, elaborated := elaborated, Assumptions, Spec, soundness, completeness }
 
 end Ragu.Circuits.Element.Square
